HAomega/EmitHaskell.lean
@@ -71,6 +71,8 @@ partial def hsTm : {Γ : List Ty} → {τ : Ty} → Tm Γ τ → Nat → String
   | _, _, .hcutH a b, d => "(hydraStep " ++ hsTm a d ++ " " ++ hsTm b d ++ ")"
   | _, _, .hleafQ a, d => "(isLeafN " ++ hsTm a d ++ ")"
   | _, _, .hordH a, d => "(ordEOfHydra " ++ hsTm a d ++ ")"
+  | _, _, .hcutAtH p a b, d =>
+      "(playAt " ++ hsTm p d ++ " " ++ hsTm a d ++ " " ++ hsTm b d ++ ")"
   | _, _, .hydra a b, d => "(hydraSeqN " ++ hsTm a d ++ " " ++ hsTm b d ++ ")"
   | _, _, .hord a, d => "(ordOfHydraN " ++ hsTm a d ++ ")"
   | _, _, .tiRec s n, d => "(tiRec " ++ hsTm s d ++ " " ++ hsTm n d ++ ")"
